src/program_proof/pav/server2.v
@@ -5,76 +5,6 @@ From Goose.github_com.mit_pdos.pav Require Import kt.
 From Perennial.program_proof.pav Require Import core cryptoffi cryptoutil serde merkle.
 From Perennial.goose_lang.lib.rwlock Require Import rwlock_noncrash.
 
-Class epoch_versioned_mapG Σ :=
-  {
-    epoch_versioned_map_histG :: mono_listG (gmap w64 (ver_ty * pk_ty)) Σ;
-    epoch_versioned_map_mapG :: ghost_mapG Σ w64 (ver_ty * pk_ty);
-  }.
-
-Section epoch_versioned_map.
-Context `{!invGS Σ}.
-Context `{!epoch_versioned_mapG Σ}.
-
-Record epoch_map_names :=
-{
-  hist_gn: gname;
-  latest_gn: gname;
-}.
-
-Implicit Type γ : epoch_map_names.
-
-(** Ownership of [uid], knowing the current version is [ver] and the current
-    public key is [pk]. *)
-Definition own_uid_dfrac γ dq (uid : w64) (ver : ver_ty) (pk : pk_ty) : iProp Σ :=
-  uid ↪[γ.(latest_gn)]{dq} (ver, pk).
-
-Notation own_uid γ uid ver pk := (own_uid_dfrac γ (DfracOwn 1) uid ver pk).
-
-(** Knowledge that the pk map at epoch [epoch] is [m]. *)
-Definition is_map γ (epoch : w64) (m : gmap w64 (ver_ty * pk_ty)) : iProp Σ :=
-  mono_list_idx_own γ.(hist_gn) (uint.nat epoch) m.
-
-Definition is_epoch_lb γ (epoch : w64) : iProp Σ :=
-  ∃ m, is_map γ epoch m.
-
-(** Ownership of the precise history of all pk maps so far. *)
-Definition own_history γ (ms : list (gmap w64 (ver_ty * pk_ty))) : iProp Σ :=
-  mono_list_auth_own γ.(hist_gn) (1/2) ms ∗
-  ghost_map_auth γ.(latest_gn) (1/2) (default ∅ (last ms)).
-
-Definition is_epoch_versioned_map γ (N : namespace) : iProp Σ :=
-  inv N (
-      ∃ ms,
-        mono_list_auth_own γ.(hist_gn) (1/2) ms ∗
-        ghost_map_auth γ.(latest_gn) (1/2) (default ∅ (last ms))
-    ).
-
-Lemma history_is_map (epoch : w64) γ ms m :
-  ms !! (uint.nat epoch) = Some m →
-  own_history γ ms -∗
-  is_map γ epoch m.
-Proof.
-Admitted.
-
-Lemma history_append {E} N (updates : gmap w64 (ver_ty * pk_ty * pk_ty)) γ ms :
-  ↑N ⊆ E →
-  own_history γ ms -∗
-  ([∗ map] uid ↦ '(ver, pk, _) ∈ updates, own_uid γ uid ver pk) ={E}=∗
-  own_history γ
-    (ms ++ [((λ '(ver, _, pk'), (word.add ver (W64 1), pk')) <$> updates) ∪ default ∅ (last ms)]) ∗
-  ([∗ map] uid ↦ '(ver, _, pk') ∈ updates, own_uid γ uid (word.add ver (W64 1)) pk').
-Proof.
-Admitted.
-
-Lemma history_agree γ ms dq uid pk ver :
-  own_history γ ms -∗
-  own_uid_dfrac γ dq uid ver pk -∗
-  ⌜ default ∅ (last ms) !! uid = Some (ver, pk) ⌝.
-Proof.
-Admitted.
-
-End epoch_versioned_map.
-
 Module userState.
 Record t :=
   mk {
@@ -145,32 +75,41 @@ Definition own_phys ptr q s : iProp Σ :=
 End defs.
 End Server.
 
+(* FIXME: remove *)
+Section auditor_defs.
+Context `{!heapGS Σ, !pavG Σ}.
+Definition audit_epoch_post (γauditor : gname) (seen_dig : list w8) : iProp Σ.
+Admitted.
+
+End auditor_defs.
+
 Section proof.
 Context `{!heapGS Σ, !pavG Σ}.
 
 Record Server_names :=
   {
-    map_gn : epoch_map_names;
+    auditor_gn : gname;
     sig_pk : list w8;
     vrf_pk : list w8;
     commitSecret : list w8;
+    epoch_gn : gname;
   }.
 
 Implicit Types γ : Server_names.
 
-(* Abstraction relation between the map in the merkle tree (which has hidden
-   labels and pks) and a map from (uid,ver) pairs to pk. *)
 Definition encode_uid_ver uid_ver :=
   (MapLabelPre.encodesF $ MapLabelPre.mk uid_ver.1 uid_ver.2).
 
 Definition encode_pk γ pk :=
   (CommitOpen.encodesF $ CommitOpen.mk pk γ.(commitSecret)).
 
+(* Abstraction relation between the map in the merkle tree (which has hidden
+   labels and pks) and a map from (uid,ver) pairs to (epoch,pk). *)
 Definition is_map_relation γ (mₗ : gmap (list w8) (list w8))
   (mₕ : gmap (uid_ty * ver_ty) (epoch_ty * pk_ty)) : iProp Σ :=
   (* A (uid_er, epoch_pk) pair is in the abstract map iff a corresponding
-     (hidden) element is in the physical map *)
-  (∀ uid_ver epoch_pk,
+     hidden element is in the physical map *)
+  □(∀ uid_ver epoch_pk,
      ⌜ mₕ !! uid_ver = Some epoch_pk ⌝ ∗-∗
      ∃ label commit,
        is_vrf_out γ.(vrf_pk) (encode_uid_ver uid_ver) label ∗
@@ -179,28 +118,23 @@ Definition is_map_relation γ (mₗ : gmap (list w8) (list w8))
 
 Context `{!epoch_versioned_mapG Σ}.
 
+(* TODO: server should own [numVers] auth to ensure cryptographic correctness. *)
+
+(* TODO: separate invariant for "ghost auditor" inside of server. *)
+
 (** Ghost ownership, invariants, and cryptographic knowledge related to mutable Server state. *)
 Definition own_Server_ghost γ st : iProp Σ :=
-  ∃ history openKeyMap (currentMap : gmap w64 (ver_ty * pk_ty)),
+  ∃ openKeyMap,
   (* abstract away the cryptographically private aspect of keyMap *)
   "#HkeyMap" ∷ is_map_relation γ st.(Server.keyMap) openKeyMap ∗
-
-  "Hhistory" ∷ own_history γ.(map_gn) history ∗
-  "%HlastHistory" ∷  ⌜ last history = Some currentMap ⌝ ∗
   "%HkeyMapLatest" ∷ (⌜ ∀ uid,
-                        match currentMap !! uid with
-                        | Some (ver, pk) =>
-                            snd <$> openKeyMap !! (uid, ver) = Some pk ∧
-                            (∀ ver', (uid, ver') ∈ dom openKeyMap ↔ uint.nat ver' ≤ uint.nat ver)
+                        match st.(Server.userInfo) !! uid with
+                        | Some (userState.mk numVers pk) =>
+                            snd <$> openKeyMap !! (uid, (word.sub numVers (W64 1))) = Some pk ∧
+                            (∀ ver, (uid, ver) ∈ dom openKeyMap ↔ uint.nat ver < uint.nat numVers)
                         | None => (∀ ver, (uid, ver) ∉ dom openKeyMap)
-                        end
-    ⌝) ∗
-
-  (* For every [userState] in [userInfo], the map has the latest value. *)
-  "%HuserState" ∷
-    (⌜ ∀ uid uinfo,
-       st.(Server.userInfo) !! uid = Some uinfo →
-       currentMap !! uid = Some ((word.sub uinfo.(userState.numVers) (W64 1)), uinfo.(userState.plainPk)) ⌝) ∗
+                        end ⌝
+    ) ∗
 
    (* Everything in epochHist is signed; could make this a crypto property of [servEpochInfo]. *)
   "#HepochHist" ∷
@@ -215,20 +149,222 @@ Definition own_Server_ghost γ st : iProp Σ :=
                           (λ v, MapValPre.encodesF (MapValPre.mk v.1 v.2)) <$>
                             (foldl union (∅ : gmap _ _)
                                (servEpochInfo.updates <$> st.(Server.epochHist)))
-                            ⌝)
+                            ⌝) ∗
+
+  "%HepochHistLast" ∷ ⌜ is_Some (last st.(Server.epochHist)) ⌝
 .
 
 (** Proposition guarded by RWMutex. *)
 Definition own_Server γ s q : iProp Σ :=
   ∃ (st : Server.t),
     "Hphys" ∷ Server.own_phys s (q/2) st ∗
-    "Hghost" ∷ own_Server_ghost γ st
-.
+    "Hghost" ∷ own_Server_ghost γ st.
 
 Definition is_Server γ s : iProp Σ :=
-  ∃ commitSecret_sl,
+  ∃ commitSecret_sl (mu vrfSk_ptr : loc),
   "#commitSecret" ∷ s ↦[Server :: "commitSecret"]□ (slice_val commitSecret_sl) ∗
   "#commitSecret_sl" ∷ own_slice_small commitSecret_sl byteT DfracDiscarded γ.(commitSecret) ∗
-  "#Hepoch_map" ∷ is_epoch_versioned_map γ.(map_gn) nroot
-  (* TODO: RWMutex invariant *)
+  "#mu" ∷ s ↦[Server :: "mu"]□ #mu ∗
+  "#Hmu" ∷ is_rwlock nroot #mu (λ q, own_Server γ s (q / 2)) ∗
+  "#vrfSk" ∷ s ↦[Server :: "vrfSk"]□ #vrfSk_ptr ∗
+  "#HvrfSk" ∷ is_vrf_sk vrfSk_ptr γ.(vrf_pk) ∗
+  "_" ∷ True
 .
+
+Definition wish_checkMembHide vrf_pk uid ver dig memb_hide label : iProp Σ :=
+  "#Hvrf_proof" ∷ is_vrf_proof vrf_pk (enc_label_pre uid ver) memb_hide.(MembHide.LabelProof) ∗
+  "#Hvrf_out" ∷ is_vrf_out vrf_pk (enc_label_pre uid ver) label ∗
+  "#Hmerk" ∷ wish_merkle_Verify true label
+    memb_hide.(MembHide.MapVal) memb_hide.(MembHide.MerkleProof) dig.
+
+Definition wish_checkMemb vrf_pk uid ver dig memb label commit : iProp Σ :=
+  "#Hvrf_proof" ∷ is_vrf_proof vrf_pk (enc_label_pre uid ver) memb.(Memb.LabelProof) ∗
+  "#Hvrf_out" ∷ is_vrf_out vrf_pk (enc_label_pre uid ver) label ∗
+  "#Hcommit" ∷ is_hash (CommitOpen.encodesF memb.(Memb.PkOpen)) commit ∗
+  "#Hmerk" ∷ wish_merkle_Verify true label
+    (enc_val memb.(Memb.EpochAdded) commit)
+    memb.(Memb.MerkleProof) dig.
+
+Definition wish_checkNonMemb vrf_pk uid ver dig non_memb : iProp Σ :=
+  ∃ label,
+  "#Hvrf_proof" ∷ is_vrf_proof vrf_pk (enc_label_pre uid ver) non_memb.(NonMemb.LabelProof) ∗
+  "#Hvrf_out" ∷ is_vrf_out vrf_pk (enc_label_pre uid ver) label ∗
+  "#Hmerk" ∷ wish_merkle_Verify false label []
+    non_memb.(NonMemb.MerkleProof) dig.
+
+Lemma wp_getDig epochHist_sl epochHist_ptrs epochHist info q :
+  last epochHist = Some info →
+  {{{
+        "HepochHist_sl" ∷ own_slice epochHist_sl ptrT (DfracOwn q) epochHist_ptrs ∗
+        "#HepochHist_own" ∷ ([∗ list] l;x ∈ epochHist_ptrs;epochHist, servEpochInfo.is_own l x)
+  }}}
+    getDig (slice_val epochHist_sl)
+  {{{
+      (sigdig_ptr : loc), RET #sigdig_ptr;
+        own_slice epochHist_sl ptrT (DfracOwn q) epochHist_ptrs ∗
+        SigDig.own sigdig_ptr (SigDig.mk (W64 (length epochHist - 1))
+                                 info.(servEpochInfo.dig)
+                                 info.(servEpochInfo.sig))
+          DfracDiscarded (* because of the slices *)
+  }}}.
+Proof.
+  intros Hlast. iIntros (?) "Hpre HΦ". iNamed "Hpre".
+  wp_rec. wp_apply wp_slice_len. iDestruct (own_slice_sz with "[$]") as %Hsz.
+  wp_pures. iDestruct (own_slice_split_1 with "[$]") as "[Hsl ?]".
+  iDestruct (big_sepL2_length with "[$]") as %Hlen_eq.
+  rewrite last_lookup in Hlast.
+  opose proof (lookup_lt_Some _ _ _ Hlast).
+  iDestruct (big_sepL2_lookup_2_some with "[$]") as %[ptr Hlookup2]; [done|].
+
+  wp_apply (wp_SliceGet with "[$Hsl]").
+  { iPureIntro. replace (uint.nat _) with (Init.Nat.pred (length epochHist)) by word.
+    eassumption. }
+  iIntros "Hsl". wp_pures.
+  iDestruct (big_sepL2_lookup with "[$]") as "H"; [eassumption.. | ].
+  iNamed "H".
+  wp_loadField. wp_loadField.
+  iApply wp_fupd.
+  wp_apply wp_allocStruct; [val_ty|].
+  iIntros "* Hl". iApply "HΦ".
+  iDestruct (struct_fields_split with "Hl") as "H". iNamed "H".
+  iMod (struct_field_pointsto_persist with "Dig") as "#Dig".
+  iMod (struct_field_pointsto_persist with "Sig") as "#Sig".
+  iMod (struct_field_pointsto_persist with "Epoch") as "#Epoch".
+  iModIntro.
+  replace (w64_word_instance.(word.sub) epochHist_sl.(Slice.sz) (W64 1)) with
+    (W64 (length epochHist - 1)) by word.
+  iFrame "∗#".
+Qed.
+
+Lemma wp_Server__Get γ ptr uid cli_ep :
+  {{{
+    "#Hserv" ∷ is_Server γ ptr ∗
+    "#Hlb_ep" ∷ mono_nat_lb_own γ.(epoch_gn) cli_ep
+  }}}
+  Server__Get #ptr #uid
+  {{{
+    ptr_sigdig sigdig sl_hist ptr2_hist hist
+    is_reg ptr_lat lat ptr_bound bound (nVers : w64),
+    RET (#ptr_sigdig, slice_val sl_hist, #ptr_lat, #ptr_bound);
+    "#Hlb_ep" ∷ mono_nat_lb_own γ.(epoch_gn) (uint.nat sigdig.(SigDig.Epoch)) ∗
+    "%Hlt_ep" ∷ ⌜ Z.of_nat cli_ep ≤ uint.Z sigdig.(SigDig.Epoch) ⌝ ∗
+    "#Hsigdig" ∷ SigDig.own ptr_sigdig sigdig DfracDiscarded ∗
+    "#Hsig" ∷ is_sig γ.(sig_pk)
+      (PreSigDig.encodesF $ PreSigDig.mk sigdig.(SigDig.Epoch) sigdig.(SigDig.Dig))
+      sigdig.(SigDig.Sig) ∗
+    "%Hlen_hist" ∷ ⌜ length hist = pred (uint.nat nVers) ⌝ ∗
+    "Hhist" ∷ ([∗ list] l;x ∈ ptr2_hist;hist,
+      MembHide.own l x (DfracOwn 1)) ∗
+    "Hsl_hist" ∷ own_slice_small sl_hist ptrT (DfracOwn 1) ptr2_hist ∗
+    "#Hwish_hist" ∷ ([∗ list] ver ↦ x ∈ hist,
+      ∃ label,
+      wish_checkMembHide γ.(vrf_pk) uid (W64 ver)
+        sigdig.(SigDig.Dig) x label) ∗
+    "Hlat" ∷ Memb.own ptr_lat lat (DfracOwn 1) ∗
+    "%Heq_is_reg" ∷ ⌜ is_reg = negb $ bool_decide (nVers = (W64 0)) ⌝ ∗
+    "#Hwish_lat" ∷ (if negb is_reg then True else
+      ∃ label commit,
+      wish_checkMemb γ.(vrf_pk) uid (word.sub nVers (W64 1))
+        sigdig.(SigDig.Dig) lat label commit) ∗
+    "Hbound" ∷ NonMemb.own ptr_bound bound (DfracOwn 1) ∗
+    "#Hwish_bound" ∷ wish_checkNonMemb γ.(vrf_pk) uid nVers sigdig.(SigDig.Dig) bound
+  }}}.
+Proof.
+  iIntros (?) "Hpre HΦ". iNamed "Hpre". iNamed "Hserv".
+  wp_rec. wp_pures. wp_loadField. wp_apply (read_wp_Mutex__Lock with "[$]").
+  iNamed 1. wp_pures.
+  iNamedSuffix "Hphys" "_own".
+  wp_loadField. wp_apply (wp_MapGet with "[$]"). iIntros "%userState_ptr %ok [%Hlookup H1_own]".
+  wp_pures. wp_apply wp_ref_of_zero; [done | ]. iIntros "%numVers_ptr numVers".
+  wp_pures. wp_apply wp_ref_of_zero; [done | ]. iIntros "%plainPk plainPk".
+  wp_pures.
+  (* TODO: optional if. *)
+  wp_if_destruct.
+  2:{
+    admit.
+  }
+  destruct ok.
+  2:{ exfalso. apply map_get_false in Hlookup. naive_solver. }
+  apply map_get_true in Hlookup.
+  iDestruct (big_sepM2_lookup_l_some with "[$]") as "%H".
+  { eassumption. }
+  destruct H as [userState Hlookup2].
+  iDestruct (big_sepM2_lookup_acc with "[$]") as "[Huinfo Huinfo_own]"; [eassumption.. | ].
+  iNamedSuffix "Huinfo" "_uinfo".
+  wp_loadField. wp_store. wp_loadField. wp_store.
+  wp_pures.
+  iCombineNamed "*_uinfo" as "Huinfo".
+  iDestruct ("Huinfo_own" with "[Huinfo]") as "Huinfo_own".
+  { iNamed "Huinfo". iFrame "∗#". }
+  iNamed "Hghost".
+  destruct HepochHistLast as [? HepochHistLast].
+  wp_loadField. wp_apply (wp_getDig with "[$]").
+  { done. }
+  iIntros (?) "[H2_own #?]". wp_pures.
+  wp_loadField. wp_load. wp_loadField.
+
+  (* TODO: wp_getHist *)
+Admitted.
+
+Lemma wp_getHist γ keyMap keyMap_ptr uid (numVers : w64) vrfSk :
+  {{{
+      own_Tree keyMap_ptr keyMap (DfracOwn 1)
+  }}}
+    getHist #keyMap_ptr #uid #numVers #vrfSk
+  {{{
+      hist hist_ptrs hist_sl, RET (slice_val hist_sl);
+      "Hhist_sl" ∷ own_slice_small hist_sl ptrT (DfracOwn 1) hist_ptrs ∗
+      "Hhist" ∷ ([∗ list] l; mh ∈ hist_ptrs; hist, MembHide.own l mh (DfracOwn 1)) ∗
+      "%Hlen_hist" ∷ ⌜ length hist = pred (uint.nat numVers) ⌝ ∗
+      "#Hwish_hist" ∷
+        (∀ dig, is_merkle_map keyMap dig -∗
+                ([∗ list] ver ↦ x ∈ hist,
+                   ∃ label, wish_checkMembHide γ.(vrf_pk) uid (W64 ver) dig x label))
+  }}}.
+Proof.
+  iIntros (?) "Hpre HΦ".
+  wp_rec. wp_pures. wp_if_destruct.
+  { (* numVers = 0 *)
+    replace (slice.nil) with (slice_val Slice.nil) by done. iApply "HΦ".
+    iDestruct (own_slice_small_nil) as "$".
+    { done. }
+    instantiate (1:=[]).
+    rewrite big_sepL2_nil.
+    iSplitR; first done.
+    iSplitR; first done.
+    iModIntro. iIntros (?) "?". done.
+  }
+  wp_pures.
+  wp_apply wp_NewSliceWithCap.
+  { word. }
+  iIntros (?) "Hhist_sl".
+  wp_apply wp_ref_to; [val_ty|].
+  iIntros (hist_ptr) "hist_ptr". wp_pures.
+  wp_apply wp_ref_to; [val_ty|].
+  iIntros (ver_ptr) "ver_ptr". wp_pures.
+
+  iAssert (
+      ∃ hist_sl hist (ver : w64) hist_ptrs,
+        "hist_ptr" ∷ hist_ptr ↦[slice.T ptrT] (slice_val hist_sl) ∗
+        "ver_ptr" ∷ ver_ptr ↦[uint64T] #ver ∗
+        "Hhist_sl" ∷ own_slice hist_sl ptrT (DfracOwn 1) hist ∗
+        "Hhist" ∷ ([∗ list] l; mh ∈ hist_ptrs; hist, MembHide.own l mh (DfracOwn 1)) ∗
+        "%Hlen_hist" ∷ ⌜ length hist = (uint.nat ver) ⌝ ∗
+        "#Hwish_hist" ∷
+          (∀ dig, is_merkle_map keyMap dig -∗
+                  ([∗ list] ver ↦ x ∈ hist,
+                     ∃ label, wish_checkMembHide γ.(vrf_pk) uid (W64 ver) dig x label))
+    )%I with "[Hhist_sl ver_ptr hist_ptr]" as "Hloop".
+  {
+    rewrite replicate_0.
+    iFrame. iExists [], []. iFrame.
+    rewrite big_sepL2_nil. iSplit; first done.
+    iSplit; first done. iIntros (?) "?". done.
+  }
+  wp_apply wp_forUpto.
+  Search For.
+  Locate "for:".
+  wp_forBreak_cond.
+Qed.
+
+End proof.
